prove locking theorems

src/program_proof/twophase/twophase_proof.v
@@ -5,16 +5,42 @@ From Perennial.program_proof Require Import lockmap_proof.
 From Perennial.program_proof Require Import addr.addr_proof buf.buf_proof.
 From Perennial.program_proof Require Import wal.abstraction.
 From Perennial.goose_lang.lib Require Import slice.typed_slice.
+From Perennial.Helpers Require Import PropRestore.
 
 Section goose_lang.
 Context `{!buftxnG Σ}.
 Context `{!heapG Σ}.
 
+(* lock addrs are all block nums only *)
+
 Definition get_mt_addrs (mt: gmap addr versioned_object) :=
-  (λ x, addr2flat (fst x)) <$> (map_to_list mt).
+  (λ x, addrBlock (fst x)) <$> (map_to_list mt).
 
 Definition get_disk_addrs (d: disk) :=
-  ((λ x, U64 (fst x)) <$> (map_to_list d)).
+  ((λ x, U64 (x.1 / (block_bytes * 8))) <$> (map_to_list d)).
+
+Definition addr_wf (dinit: disk) a :=
+  is_Some (dinit !! (addr2flat_z a)) ∧ int.Z (addrOff a) < block_bytes * 8.
+
+Definition addr_wf' (dinit: disk) a :=
+  (addrBlock a) ∈ get_disk_addrs dinit ∧ int.Z (addrOff a) < block_bytes * 8.
+
+Lemma addr_wf_wf' dinit a:
+  addr_wf dinit a → addr_wf' dinit a.
+Proof.
+  intros [Hblk Hoff].
+  split.
+  2: assumption.
+  rewrite /get_disk_addrs.
+  destruct Hblk as [b Hb].
+  eapply elem_of_list_fmap_1_alt.
+  1: apply elem_of_map_to_list; apply Hb.
+  rewrite /addr2flat_z /addrBlock /=.
+  rewrite -Z.mul_assoc Z.div_add_l.
+  2: auto.
+  rewrite Zdiv_small.
+  all: word.
+Qed.
 
 Definition is_twophase_inner (l : loc) mt (locked_addrs: list u64) γ (dinit: disk) : iProp Σ := (
   ∃ (buftxnl locksl: loc) acquired_s anydirty ghs (dinit_addrs: gset u64) (acquired: list u64),
@@ -25,8 +51,8 @@ Definition is_twophase_inner (l : loc) mt (locked_addrs: list u64) γ (dinit: di
     "Htwophase.acquired" ∷ l ↦[TwoPhase.S :: "acquired"] (slice_val acquired_s) ∗
     "Hbuftxn" ∷ is_buftxn buftxnl mt γ dinit anydirty ∗
     "#Hlocks" ∷ is_lockMap locksl ghs (list_to_set dinit_addrs) (const True%I) ∗
-    "Hacquired_s" ∷ is_slice acquired_s uint64T 1 mt_addrs ∗
-    "Hlocked_addrs" ∷ [∗ list] a ∈ locked_addrs, Locked ghs a ∗
+    "Hacquired_s" ∷ is_slice acquired_s uint64T 1 locked_addrs ∗
+    "Hlocked_addrs" ∷ ([∗ list] a ∈ locked_addrs, Locked ghs a) ∗
     "%Hmt_addrs_locked" ∷ ⌜mt_addrs ⊆ locked_addrs⌝ ∗
     "%Hlocked_addrs_wf" ∷ ⌜locked_addrs ⊆ dinit_addrs⌝
 )%I.
@@ -70,10 +96,14 @@ Proof.
   wp_apply util_proof.wp_DPrintf.
   wp_pures.
   iApply "HΦ".
-  iExists _, _, _, _, _, _, _.
   iDestruct (struct_fields_split with "Hl") as "(Htwophase.buftxn & Htwophase.locks & Htwophase.acquired & %)".
+  iExists _, _, _, _, _, _, _.
   rewrite /get_mt_addrs /get_disk_addrs map_to_list_empty /=.
   iFrame "# ∗".
+  iSplit; first by auto.
+  iSplit; first by auto.
+  iPureIntro.
+  apply list_subseteq_nil.
   Unshelve.
   - apply ∅.
   - apply [].
@@ -81,56 +111,254 @@ Qed.
 
 Theorem wp_twophase__Acquire (l: loc) mt locked_addrs γ dinit a:
   {{{
-    is_twophase_inner l mt locked_addrs γ dinit
+    "Htwophase" ∷ is_twophase_inner l mt locked_addrs γ dinit ∗
+    "%Ha_wf" ∷ ⌜addr_wf dinit a⌝
   }}}
     TwoPhase__Acquire #l (addr2val a)
   {{{
-    (l : loc), RET #l;
-    let flata := addr2flat a in
-    if (decide (flata ∈ locked_addrs)) then
-      is_twophase_inner l mt locked_addrs γ dinit
-    else
-      is_twophase_inner l mt (locked_addrs ++ [addr2flat a]) γ dinit
+    RET #();
+    let blk := addrBlock a in
+    let locked_addrs' := if (decide (blk ∈ locked_addrs)) then
+        locked_addrs else locked_addrs ++ [blk] in
+    is_twophase_inner l mt locked_addrs' γ dinit
   }}}.
 Proof.
   wp_start.
   wp_call.
-  wp_apply wp_ref_to; first by eauto.
+  wp_apply wp_ref_to; first by auto.
   iIntros (already_acquired_l) "Halready_acquired_l".
-  wp_pures.
-  iNamed "Hpre".
+  iNamed "Htwophase".
   wp_loadField.
   iDestruct (is_slice_small_read with "Hacquired_s") as "[Hacquired_s Hacquired_s_wrap]".
-  destruct (decide (addr2flat a ∈ locked_addrs)).
-  {
-    wp_apply (wp_forSlice (λ _,
-      "Halready_acquired_l" ∷ already_acquired_l ↦[boolT] #false
-    )%I with "[] [Hacquired_s $Halready_acquired_l]").
-    2: admit.
-    {
-      iIntros (i x Φ0).
-      iModIntro.
-      iNamed 1.
-      iIntros "HΦ".
-      wp_pures.
-      iApply "HΦ".
-      iFrame.
-    }
-    iIntros "[Halready_acquired_l Hacquired_s]".
-    wp_pures.
-    admit.
+  wp_apply (wp_forSlicePrefix (λ done todo,
+    let already_acquired_val := bool_decide (addrBlock a ∈ done) in
+    "Halready_acquired_l" ∷ already_acquired_l ↦[boolT] #already_acquired_val
+  )%I (V:=u64) with "[] [$Hacquired_s Halready_acquired_l]").
+  2: {
+    rewrite bool_decide_eq_false_2; first by iFrame.
+    apply not_elem_of_nil.
   }
-  admit.
-Admitted.
+  {
+    iIntros (i x done todo Harr Φ0).
+    iModIntro.
+    iNamed 1.
+    iIntros "HΦ".
+    wp_if_destruct.
+    {
+      wp_apply (wp_StoreAt with "[$Halready_acquired_l]").
+      1: auto.
+      iIntros "Halready_acquired_l".
+      iApply "HΦ".
+      rewrite bool_decide_eq_true_2; first by iFrame.
+      apply elem_of_app.
+      right.
+      apply (iffRL (elem_of_list_singleton _ _)).
+      reflexivity.
+    }
+    iApply "HΦ".
+    destruct (decide (addrBlock a ∈ done)).
+    - rewrite bool_decide_eq_true_2.
+      2: assumption.
+      rewrite bool_decide_eq_true_2; first by iFrame.
+      apply elem_of_app.
+      left.
+      assumption.
+    - rewrite bool_decide_eq_false_2.
+      2: assumption.
+      rewrite bool_decide_eq_false_2; first by iFrame.
+      apply not_elem_of_app.
+      split; first by assumption.
+      intro Hin.
+      apply elem_of_list_singleton in Hin.
+      apply Heqb.
+      f_equal.
+      f_equal.
+      apply Hin.
+  }
+  iIntros "[Hacquired_s ?]".
+  iNamed.
+  iApply "Hacquired_s_wrap" in "Hacquired_s".
+  wp_apply (wp_LoadAt with "[$Halready_acquired_l]").
+  iIntros "Halready_acquired_l".
+  wp_if_destruct.
+  2: {
+    iApply "HΦ".
+    rewrite decide_True.
+    2: assumption.
+    iExists _, _, _, _, _, _, _.
+    iFrame "∗ # %".
+  }
+  rewrite bool_decide_eq_false_2.
+  2: assumption.
+  wp_loadField.
+  apply addr_wf_wf' in Ha_wf.
+  wp_apply (wp_LockMap__Acquire with "[$Hlocks]").
+  {
+    iPureIntro.
+    apply elem_of_list_to_set.
+    destruct Ha_wf.
+    intuition.
+  }
+  iIntros "[_ Hlocked]".
+  wp_loadField.
+  wp_apply (wp_SliceAppend (V:=u64) with "[$Hacquired_s]").
+  iIntros (acquired_s') "Hacquired_s".
+  wp_apply (wp_storeField with "Htwophase.acquired").
+  1: rewrite /field_ty /=; val_ty.
+  iIntros "Htwophase.acquired".
+  iApply "HΦ".
+  rewrite decide_False.
+  2: assumption.
+  iExists _, _, _, _, _, _, _.
+  iFrame "∗ #".
+  iSplit; first by auto.
+  destruct Ha_wf.
+  iSplit; iPureIntro; set_solver.
+  Unshelve.
+  all: auto.
+Qed.
 
-Theorem wp_twophase__ReleaseAll (l: loc) mt locked_addrs γ dinit:
+Theorem wp_twophase__Release (l: loc) locked_addrs a γ dinit:
   {{{
-    is_twophase_inner l mt locked_addrs γ dinit
+    is_twophase_inner l ∅ (locked_addrs ++ [a]) γ dinit
+  }}}
+    TwoPhase__Release #l
+  {{{
+    RET #();
+    is_twophase_inner l ∅ locked_addrs γ dinit
+  }}}.
+Proof.
+  wp_start.
+  wp_call.
+  iNamed "Hpre".
+  wp_loadField.
+  wp_apply wp_slice_len.
+  wp_loadField.
+  iDestruct (is_slice_small_read with "Hacquired_s") as "[Hacquired_s Hacquired_s_wrap]".
+  iDestruct (is_slice_small_sz with "Hacquired_s") as "%Hacquired_s_sz".
+  assert ((locked_addrs ++ [a]) !! (length locked_addrs) = Some a) as Hlocked_addrs_acc.
+  {
+    rewrite lookup_app_r.
+    2: lia.
+    rewrite Nat.sub_diag //.
+  }
+  rewrite app_length /= in Hacquired_s_sz.
+  assert (int.nat acquired_s.(Slice.sz) > 0) as Hacquired_s_sz_gt by lia.
+  wp_apply (wp_SliceGet (V:=u64) with "[$Hacquired_s]").
+  {
+    iPureIntro.
+    replace (int.nat (word.sub _ 1)) with ((int.nat acquired_s.(Slice.sz)) - 1)%nat by word.
+    rewrite -Hacquired_s_sz Nat.add_sub.
+    apply Hlocked_addrs_acc.
+  }
+  iIntros "Hacquired_s".
+  wp_loadField.
+  iDestruct (big_sepL_app with "Hlocked_addrs") as "[Hlocked_addrs Hlocked]".
+  rewrite big_sepL_singleton.
+  wp_apply (wp_LockMap__Release with "[$Hlocks $Hlocked //]").
+  wp_loadField.
+  wp_apply (wp_SliceTake uint64T).
+  1: word.
+  wp_apply (wp_storeField with "Htwophase.acquired").
+  1: rewrite /field_ty /=; val_ty.
+  iIntros "Htwophase.acquired".
+  iApply "HΦ".
+  iExists _, _, _, _, _, _, _.
+  iApply "Hacquired_s_wrap" in "Hacquired_s".
+  iFrame "∗ #".
+  iSplitL "Hacquired_s".
+  {
+    iApply (is_slice_take_cap _ _ _ (word.sub acquired_s.(Slice.sz) 1)) in "Hacquired_s".
+    1: rewrite fmap_length app_length /=; word.
+    replace (int.nat (word.sub _ 1)) with ((int.nat acquired_s.(Slice.sz)) - 1)%nat by word.
+    rewrite -fmap_take -Hacquired_s_sz Nat.add_sub take_app.
+    iFrame.
+  }
+  rewrite /get_mt_addrs map_to_list_empty /=.
+  iSplit; iPureIntro; set_solver.
+  Unshelve.
+  all: auto.
+Qed.
+
+Theorem wp_twophase__ReleaseAll (l: loc) locked_addrs γ dinit:
+  {{{
+    is_twophase_inner l ∅ locked_addrs γ dinit
   }}}
     TwoPhase__ReleaseAll #l
   {{{
     RET #();
-    is_twophase_inner l mt [] γ dinit
+    is_twophase_inner l ∅ [] γ dinit
   }}}.
 Proof.
-Admitted.
+  wp_start.
+  wp_call.
+  Check wp_forBreak_cond.
+  wp_apply (wp_forBreak_cond (λ b,
+    ∃ locked_addrs',
+      "Htwophase" ∷ is_twophase_inner l ∅ locked_addrs' γ dinit ∗
+      "%Hb" ∷ ⌜b = false → locked_addrs' = []⌝
+  )%I with "[] [Hpre]").
+  2: {
+    iExists (locked_addrs).
+    iFrame.
+    auto.
+  }
+  {
+    iModIntro.
+    iIntros (Φ') "Hloop HΦ'".
+    clear locked_addrs.
+    iDestruct "Hloop" as (locked_addrs) "[? ?]".
+    iNamed.
+    iNamed "Htwophase".
+    wp_loadField.
+    wp_apply wp_slice_len.
+    iDestruct (is_slice_sz with "Hacquired_s") as "%Hlocked_addrs_len".
+    wp_if_destruct.
+    2: {
+      iApply "HΦ'".
+      iExists locked_addrs.
+      rewrite Heqb in Hlocked_addrs_len.
+      replace (int.nat 0) with 0%nat in Hlocked_addrs_len by word.
+      apply nil_length_inv in Hlocked_addrs_len.
+      subst locked_addrs.
+      iSplitL.
+      2: auto.
+      iExists _, _, _, _, _, _, _.
+      iFrame "∗ #".
+      rewrite /get_mt_addrs map_to_list_empty //=.
+    }
+    iAssert (is_twophase_inner l ∅ locked_addrs γ dinit) with
+      "[Htwophase.buftxn Htwophase.locks Htwophase.acquired
+      Hbuftxn Hacquired_s Hlocked_addrs]"
+    as "Htwophase".
+    {
+      iExists _, _, _, _, _, _, _.
+      iFrame "∗ # %".
+    }
+    apply u64_val_ne in Heqb.
+    replace (int.Z 0) with 0 in Heqb by word.
+    assert (int.nat acquired_s.(Slice.sz) ≠ 0%nat) as Hacquired_s_sz by word.
+    rewrite -Hlocked_addrs_len in Hacquired_s_sz.
+    assert (0 < length locked_addrs)%nat as Hlocked_addrs by lia.
+    apply length_nonzero_neq_nil in Hlocked_addrs.
+    apply exists_last in Hlocked_addrs.
+    destruct Hlocked_addrs as (locked_addrs'&locked_tail&->).
+    wp_apply (wp_twophase__Release with "Htwophase").
+    iIntros "Htwophase".
+    wp_pures.
+    iApply "HΦ'".
+    iExists _.
+    iFrame.
+    auto.
+    Unshelve.
+    all: auto.
+  }
+  iIntros "Hloop".
+  clear locked_addrs.
+  iDestruct "Hloop" as (locked_addrs) "[? ?]".
+  iNamed.
+  pose proof (Hb eq_refl) as Hlocked_addrs.
+  subst.
+  iApply "HΦ".
+  iFrame.
+Qed.
